fix MutrecA spec

demo/mutrec/static_a.c
@@ -5,7 +5,7 @@ static int memoized[10] = {-1, -1, -1, -1, -1, -1, -1, -1, -1, -1};
 int f(int x) {
   if(x == 0) return 0;
   if(memoized[x] < 0) {
-    memoized[x] = g(x-1) + x-1;
+    memoized[x] = g(x-1) + x;
   }
   return memoized[x];
 }
