demo/mutrec/StaticMutrecAproof.v
@@ -11,20 +11,404 @@ Require Import StaticMutrecA StaticMutrecAspec.
 Require Import Simulation.
 Require Import Skeleton Mod ModSem SimMod SimModSem SimSymb SimMem AsmregsC MatchSimModSem.
 (* Require SimMemInjC. *)
-Require SimMemId.
 Require SoundTop.
+Require SimMemInjInv.
 Require Import Clightdefs.
 Require Import CtypesC.
 
 Set Implicit Arguments.
 
-Theorem sim_mod
+Print Instances SimMem.class.
+
+
+Definition memoized_inv (chunk: memory_chunk) (ofs: Z) (v: option val): Prop :=
+  forall
+    ind
+    (BOUND: 0 <= ind < 10)
+    (INT: chunk = Mint64)
+    (INDEX: size_chunk Mint64 * ind = ofs),
+  exists i,
+    (<<VAL: v = Some (Vint i)>>) /\
+    forall (VPOS: 0 <= i.(Int.intval)),
+      i = sum (Int.repr ind).
+
+Local Instance SimMemMemoized: SimMem.class := SimMemInjInv.SimMemInjInv memoized_inv.
+
+Definition symbol_memoized: ident -> Prop := eq _memoized.
+
+Section SIMMODSEM.
+
+Variable skenv_link: SkEnv.t.
+Variable sm_link: SimMem.t.
+Let md_src: Mod.t := (StaticMutrecAspec.module).
+Let md_tgt: Mod.t := (ClightC.module2 prog).
+Hypothesis (INCL: SkEnv.includes skenv_link md_src.(Mod.sk)).
+Hypothesis (WF: SkEnv.wf skenv_link).
+Let ge := (SkEnv.project skenv_link md_src.(Mod.sk)).
+Let tge := Build_genv (SkEnv.revive (SkEnv.project skenv_link md_tgt.(Mod.sk)) prog) prog.(prog_comp_env).
+Definition msp: ModSemPair.t :=
+  ModSemPair.mk (md_src skenv_link) (md_tgt skenv_link) symbol_memoized sm_link.
+
+
+Inductive match_states_internal: StaticMutrecAspec.state -> Clight.state -> Prop :=
+| match_callstate_nonzero
+    i m_src m_tgt
+    fptr
+    (* targs tres cconv *)
+    (FINDF: Genv.find_funct (Smallstep.globalenv (modsem2 skenv_link prog)) fptr = Some (Internal func_f))
   :
-    ModPair.sim (ModPair.mk (StaticMutrecAspec.module) (ClightC.module2 prog) tt)
+    match_states_internal (Callstate i m_src) (Clight.Callstate fptr (Tfunction (* targs tres cconv) *)
+                                                                        (Tcons tint Tnil) tint cc_default)
+                                                                [Vint i] Kstop m_tgt)
+| match_returnstate
+    i m_src m_tgt
+  :
+    match_states_internal (Returnstate i m_src) (Clight.Returnstate (Vint i) Kstop m_tgt)
+.
+
+
+(* Inductive match_states_internal: StaticMutrecAspec.state -> Clight.state -> Prop := *)
+(* | match_callstate_nonzero_memoized *)
+(*     i m_src m_tgt *)
+(*     fptr blk memov *)
+(*     (* targs tres cconv *) *)
+(*     (FINDF: Genv.find_funct (Smallstep.globalenv (modsem2 skenv_link prog)) fptr = Some (Internal func_f)) *)
+(*     (SYMB: Genv.find_symbol skenv_link _memoized = Some blk) *)
+(*     (MEMOLD: Mem.loadv *)
+(*                Mint64 m_tgt *)
+(*                (Vptr blk (Ptrofs.repr (size_chunk Mint64 * i.(Int.intval)))) = Some (Vint memov)) *)
+(*     (MEMOIZED: memov = sum i) *)
+(*   : *)
+(*     match_states_internal (Callstate i m_src) (Clight.Callstate fptr (Tfunction (* targs tres cconv) *) *)
+(*                                                                         (Tcons tint Tnil) tint cc_default) *)
+(*                                                                 [Vint i] Kstop m_tgt) *)
+(* | match_callstate_nonzero_nonmemoized *)
+(*     i m_src m_tgt *)
+(*     fptr blk memov *)
+(*     (* targs tres cconv *) *)
+(*     (FINDF: Genv.find_funct (Smallstep.globalenv (modsem2 skenv_link prog)) fptr = Some (Internal func_f)) *)
+(*     (SYMB: Genv.find_symbol skenv_link _memoized = Some blk) *)
+(*     (MEMOLD: Mem.loadv *)
+(*                Mint64 m_tgt *)
+(*                (Vptr blk (Ptrofs.repr (size_chunk Mint64 * i.(Int.intval)))) = Some (Vint memov)) *)
+(*     (NONMEMOIZED: memov.(Int.intval) < 0) *)
+(*   : *)
+(*     match_states_internal (Callstate i m_src) (Clight.Callstate fptr (Tfunction (* targs tres cconv) *) *)
+(*                                                                         (Tcons tint Tnil) tint cc_default) *)
+(*                                                                 [Vint i] Kstop m_tgt) *)
+(* | match_returnstate *)
+(*     i m_src m_tgt *)
+(*   : *)
+(*     match_states_internal (Returnstate i m_src) (Clight.Returnstate (Vint i) Kstop m_tgt) *)
+(* . *)
+
+Inductive match_states (sm_init: SimMem.t)
+          (idx: nat) (st_src0: StaticMutrecAspec.state) (st_tgt0: Clight.state) (sm0: SimMem.t): Prop :=
+| match_states_intro
+    (MATCHST: match_states_internal st_src0 st_tgt0)
+    (MCOMPATSRC: st_src0.(get_mem) = sm0.(SimMem.src))
+    (MCOMPATTGT: st_tgt0.(ClightC.get_mem) = sm0.(SimMem.tgt))
+    (MWF: SimMem.wf sm0)
+    (IDX: (idx > 3)%nat)
+.
+
+Lemma g_blk_exists
+  :
+    exists g_blk,
+      (<<FINDG: Genv.find_symbol
+                  (SkEnv.revive (SkEnv.project skenv_link (CSk.of_program signature_of_function prog)) prog)
+                  g_id = Some g_blk>>)
+      /\
+      (<<FINDG: Genv.find_funct_ptr
+                  (SkEnv.revive (SkEnv.project skenv_link (CSk.of_program signature_of_function prog)) prog)
+                  g_blk = None>>)
+      /\
+      (<<FINDG: exists skd, Genv.find_funct_ptr skenv_link g_blk = Some skd /\
+                            signature_of_type (Tcons tint Tnil) tint cc_default = SkEnv.get_sig skd>>)
 .
 Proof.
-  econs; ss.
-  - ii. inv SIMSKENVLINK.
-    admit "".
-    (* eapply sim_modsem; eauto. *)
+  exploit (prog_defmap_norepet prog g_id); eauto.
+  { unfold prog_defs_names. ss. repeat (econs; eauto).
+    - ii; ss; des; ss.
+    - ii; ss; des; ss. }
+  { ss. eauto. }
+  intro T; des.
+  exploit SkEnv.project_impl_spec; eauto. intro PROJ.
+  assert(PREC: SkEnv.genv_precise
+                 (SkEnv.revive (SkEnv.project skenv_link (CSk.of_program signature_of_function prog)) prog)
+                 prog).
+  { eapply CSkEnv.project_revive_precise; ss; et. }
+  inv PREC.
+  exploit (P2GE g_id); eauto. i; des. des_ifs.
+  rename b into g_blk.
+  eexists. splits; et.
+  { unfold Genv.find_funct_ptr. des_ifs. }
+  (* exploit (@SkEnv.project_revive_precise _ _ skenv_link); eauto. *)
+  { inv INCL.
+    exploit (CSk.of_program_prog_defmap prog signature_of_function); et. rewrite T. intro S.
+
+    remember ((prog_defmap (CSk.of_program signature_of_function prog)) ! g_id) as U in *.
+    destruct U eqn:V; try (by ss). inv S. inv H1.
+
+    exploit DEFS; eauto. i; des.
+    assert(blk = g_blk).
+    { inv PROJ. exploit SYMBKEEP; et.
+      - instantiate (1:= g_id). unfold defs. des_sumbool. ss. et.
+      - i. rewrite SYMB0 in *. clear - SYMB H. unfold SkEnv.revive in *. rewrite Genv_map_defs_symb in *. ss.
+        rewrite SYMB in *. des. clarify.
+    }
+    clarify. inv MATCH.
+    esplits; eauto.
+    - unfold Genv.find_funct_ptr. rewrite DEF0. et.
+    - ss. des_ifs. clear - H1. inv H1; ss.
+  }
 Qed.
+
+Lemma match_states_lxsim
+      sm_init idx st_src0 st_tgt0 sm0
+      (MATCH: match_states sm_init idx st_src0 st_tgt0 sm0)
+  :
+    <<XSIM: lxsim (md_src skenv_link) (md_tgt skenv_link)
+                  (fun st => exists su m_init, SoundTop.sound_state su m_init st)
+                  sm_init (Ord.lift_idx lt_wf idx) st_src0 st_tgt0 sm0>>
+.
+Proof.
+  revert_until tge.
+  pcofix CIH.
+  i.
+  pfold.
+  generalize g_blk_exists; et. i; des.
+  inv MATCH. ss. inv MATCHST; ss; clarify.
+  - (* call *)
+    destruct (classic (i = Int.zero)).
+    + (* zero *)
+      clarify.
+      econs 2. i. esplits; cycle 3.
+      { ii. esplits. econs; eauto. econs; ss; eauto.
+        - econs.
+        - econs; eauto. econs.
+        - ii. ss. des; clarify.
+        - econs. }
+      { ii. inv H. inv H0. }
+      { ii. inv H. inv H0. }
+      econs 2.
+      { split.
+        - econs 2.
+          + ss. econs 1.
+          + econs 1.
+          + ss.
+        - admit "index". }
+      left. pfold.
+      econs 1. i; des.
+      econs 2.
+
+      (* econs 2; cycle 2. *)
+      (* { admit "ez - spec is receptive". } *)
+      (* { split; ii; rr in H; inv H; inv H0; ss. } *)
+      (* i. ss. inv STEPSRC. *)
+      (* esplits; eauto. *)
+
+      * split; cycle 1.
+        { admit "index". }
+
+        (* left. *)
+        eapply plus_left with (t1 := E0) (t2 := E0); ss.
+        { econs; eauto.
+          { eapply modsem2_determinate; eauto. }
+          econs; eauto.
+          econs; ss; eauto; try (by repeat (econs; ss; eauto)).
+          unfold _x. unfold _t'1. rr. ii; ss. des; ss. clarify.
+        }
+
+        eapply star_left with (t1 := E0) (t2 := E0); ss.
+        { econs; eauto.
+          { eapply modsem2_determinate; eauto. }
+          econs; eauto.
+        }
+
+        eapply star_left with (t1 := E0) (t2 := E0); ss.
+        { econs; eauto.
+          { eapply modsem2_determinate; eauto. }
+          econs; eauto.
+          - repeat econs; et.
+          - ss.
+        }
+
+        eapply star_left with (t1 := E0) (t2 := E0); ss.
+        { econs; eauto.
+          { eapply modsem2_determinate; eauto. }
+          econs; eauto.
+          - repeat econs; et.
+          - ss.
+          - ss.
+        }
+
+        apply star_refl.
+      (* * refl. *)
+      * right. eapply CIH. econs; ss; eauto.
+        replace (Int.repr 0) with (sum Int.zero).
+        { econs; eauto. }
+        { admit "". }
+
+    + (* nonzero *)
+
+      destruct sm0.
+      destruct (Genv.find_symbol skenv_link _memoized) eqn:BLK; cycle 1.
+      { exfalso. clear - INCL BLK. inv INCL.
+        exploit DEFS; eauto.
+        - instantiate (2:=_memoized). ss.
+        - i. des. clarify. }
+
+      inv MWF. ss. admit "".
+      (* exploit SAT. *)
+
+  - admit "".
+    Unshelve. all : admit "".
+
+(*       destruct (Mem.loadv *)
+(*                   Mint64 (minj.(SimMemInj.tgt)) *)
+(*                   (Vptr b (Ptrofs.repr (size_chunk Mint64 * i.(Int.intval))))). *)
+
+(*       Mem.loadv *)
+(*                    Mint64 m_tgt *)
+(*                    (Vptr blk (Ptrofs.repr (size_chunk Mint64 * i.(Int.intval)))) *)
+
+
+(*       (MEMOLD: Mem.loadv *)
+(*                    Mint64 m_tgt *)
+(*                    (Vptr blk (Ptrofs.repr (size_chunk Mint64 * i.(Int.intval)))) = Some (Vint memov)) *)
+(*         (MEMOIZED: memov = sum i) *)
+
+
+
+
+
+(*       econs. *)
+(*       i; des. *)
+(*       econs 2; eauto. *)
+(*       * esplits; cycle 1. *)
+(*         { eapply Ord.lift_idx_spec. instantiate (1:= 2%nat). lia. } *)
+
+(*         eapply plus_left with (t1 := E0) (t2 := E0); ss. *)
+(*         { econs; eauto. *)
+(*           { eapply modsem2_determinate; eauto. } *)
+(*           econs; eauto. *)
+(*           econs; ss; eauto; try (by repeat (econs; ss; eauto)). *)
+(*           unfold _x. unfold _t'1. rr. ii; ss. des; ss. clarify. *)
+(*         } *)
+
+(*         eapply star_left with (t1 := E0) (t2 := E0); ss. *)
+(*         { econs; eauto. *)
+(*           { eapply modsem2_determinate; eauto. } *)
+(*           econs; eauto. *)
+(*         } *)
+
+(*         eapply star_left with (t1 := E0) (t2 := E0); ss. *)
+(*         { econs; eauto. *)
+(*           { eapply modsem2_determinate; eauto. } *)
+(*           econs; eauto. *)
+(*           - repeat econs; et. *)
+(*           - ss. rewrite Int.eq_false; ss. *)
+(*         } *)
+
+(*         eapply star_left with (t1 := E0) (t2 := E0); ss. *)
+(*         { econs; eauto. *)
+(*           { eapply modsem2_determinate; eauto. } *)
+(*           econs; eauto. *)
+(*         } *)
+
+(*         eapply star_left with (t1 := E0) (t2 := E0); ss. *)
+(*         { econs; eauto. *)
+(*           { eapply modsem2_determinate; eauto. } *)
+(*           econs; eauto. *)
+(*         } *)
+
+(*         eapply star_left with (t1 := E0) (t2 := E0); ss. *)
+(*         { econs; eauto. *)
+(*           { eapply modsem2_determinate; eauto. } *)
+(*           econs; eauto; swap 1 2. *)
+(*           - econs. *)
+(*             + eapply eval_Evar_global; ss. et. *)
+(*             + econs 2; et. *)
+(*           - unfold Cop.classify_fun. ss. *)
+(*           - repeat econs; ss; et. *)
+(*         } *)
+
+(*         apply star_refl. *)
+(*       * left. pfold. econs 3; et. *)
+(*         { rr. esplits; eauto. ss. econs; et. ii. destruct i; ss. clarify. apply H. unfold Int.zero. *)
+(*           Local Transparent Int.repr. *)
+(*           unfold Int.repr. *)
+(*           Local Opaque Int.repr. *)
+(*           ss. apply eta; ss. *)
+(*         } *)
+(*         ii; des. *)
+(*         inv ATSRC. ss; clarify. *)
+(*         destruct sm0; ss. clarify. *)
+(*         unfold Clight.fundef in *. *)
+(*         assert(g_fptr = g_blk). *)
+(*         { unfold SkEnv.revive in FINDG. rewrite Genv_map_defs_symb in *. clarify. } *)
+(*         clarify. *)
+(*         eexists (Args.mk _ [Vint (Int.sub i (Int.repr 1))] _), (SimMemId.mk _ _). *)
+(*         esplits; ss; eauto. *)
+(*         { econs; ss; eauto. } *)
+(*         i. inv AFTERSRC. destruct retv_src, retv_tgt; ss. clarify. destruct sm_ret; ss. inv SIMRETV; ss; clarify. *)
+(*         esplits; eauto. *)
+(*         { econs; eauto. } *)
+(*         instantiate (2:= (Ord.lift_idx lt_wf 15%nat)). *)
+(*         left. pfold. econs; eauto. i; des. econs 2; eauto. *)
+(*         { *)
+(*           esplits; eauto; cycle 1. *)
+(*           { instantiate (1:= (Ord.lift_idx lt_wf 14%nat)). eapply Ord.lift_idx_spec; et. } *)
+
+(*           eapply plus_left with (t1 := E0) (t2 := E0); ss. *)
+(*           { econs; eauto. *)
+(*             { eapply modsem2_determinate; eauto. } *)
+(*             econs; eauto. *)
+(*           } *)
+
+(*           eapply star_left with (t1 := E0) (t2 := E0); ss. *)
+(*           { econs; eauto. *)
+(*             { eapply modsem2_determinate; eauto. } *)
+(*             econs; eauto. *)
+(*           } *)
+
+(*           eapply star_left with (t1 := E0) (t2 := E0); ss. *)
+(*           { econs; eauto. *)
+(*             { eapply modsem2_determinate; eauto. } *)
+(*             econs; ss; eauto. *)
+(*             - repeat (econs; ss; eauto). *)
+(*               + unfold typify. des_ifs. *)
+(*             - ss. *)
+(*           } *)
+
+(*           eapply star_refl. *)
+(*         } *)
+
+(*         right. eapply CIH. instantiate (1:= SimMemId.mk _ _). *)
+(*         econs; ss; eauto; try lia. *)
+(*         rewrite sum_recurse. des_ifs. *)
+(*         { rewrite Z.eqb_eq in *. lia. } *)
+(*         replace (Int.sub (Int.add (sum (Int.sub i Int.one)) i) (Int.repr 1)) with *)
+(*             (Int.add (sum (Int.sub i Int.one)) (Int.sub i Int.one)); cycle 1. *)
+(*         { abstr (sum (Int.sub i Int.one)) z. rewrite ! Int.sub_add_opp. *)
+(*           rewrite Int.add_assoc. ss. } *)
+(*         econs; eauto. *)
+(*   - (* return *) *)
+(*     econs 4; ss; eauto. *)
+(* Unshelve. *)
+(*   all: ss. *)
+Qed.
+
+End SIMMODSEM.
+
+
+Theorem sim_mod
+  :
+    ModPair.sim (ModPair.mk (StaticMutrecAspec.module) (ClightC.module2 prog) symbol_memoized)
+.
+Proof.
+Admitted.
+(*   econs; ss. *)
+(*   - ii. inv SIMSKENVLINK. *)
+(* Qed. *)
